Work on trace approximation

Equiv/TraceEquiv.v
@@ -6,30 +6,30 @@ Set Implicit Arguments.
 Unset Printing Records.
 
 Inductive extevent :=
-  | EEvt (evt:event)
-  | EvtTerminate (res:option val).
+  | EEvtExtern (evt:event)
+  | EEvtTerminate (res:option val).
 
-Inductive produces_prefix {S} `{StateType S} : S -> list extevent -> Prop :=
+Inductive prefix {S} `{StateType S} : S -> list extevent -> Prop :=
   | producesPrefixSilent (σ:S) (σ':S) L :
       step σ EvtTau σ'
-      -> produces_prefix σ' L
-      -> produces_prefix σ  L
+      -> prefix σ' L
+      -> prefix σ  L
   | producesPrefixExtern (σ:S) (σ':S) evt L :
       activated σ
       -> step σ evt σ'
-      -> produces_prefix σ' L
-      -> produces_prefix σ (EEvt evt::L)
+      -> prefix σ' L
+      -> prefix σ (EEvtExtern evt::L)
   | producesPrefixTerm (σ:S) (σ':S) r
     : result σ' = r
       -> star2 step σ nil σ'
       -> normal2 step σ'
-      -> produces_prefix σ (EvtTerminate r::nil)
+      -> prefix σ (EEvtTerminate r::nil)
   | producesPrefixPrefix (σ:S)
-    : produces_prefix σ nil.
+    : prefix σ nil.
 
-Lemma produces_prefix_star2_silent {S} `{StateType S} (σ σ':S) L
+Lemma prefix_star2_silent {S} `{StateType S} (σ σ':S) L
  : star2 step σ nil σ' ->
-   produces_prefix σ' L -> produces_prefix σ L.
+   prefix σ' L -> prefix σ L.
 Proof.
   intros. general induction H0; eauto.
   - destruct yl, y; simpl in *; try congruence.
@@ -47,9 +47,9 @@ Proof.
 Qed.
 
 
-Lemma produces_prefix_star2_silent' {S} `{StateType S} (σ σ':S) L
+Lemma prefix_star2_silent' {S} `{StateType S} (σ σ':S) L
  : star2 step σ nil σ' ->
-   produces_prefix σ L -> produces_prefix σ' L.
+   prefix σ L -> prefix σ' L.
 Proof.
   intros. general induction H0; eauto.
   - destruct yl, y; simpl in *; try congruence.
@@ -76,21 +76,21 @@ Proof.
 Qed.
 
 Lemma bisim_prefix {S} `{StateType S} {S'} `{StateType S'} (sigma:S) (σ':S')
-: bisim sigma σ' -> forall L, produces_prefix sigma L -> produces_prefix σ' L.
+: bisim sigma σ' -> forall L, prefix sigma L -> prefix σ' L.
 Proof.
   intros. general induction H2.
   - eapply bisim_bisim' in H3.
-    eapply IHproduces_prefix; eauto.
+    eapply IHprefix; eauto.
     eapply bisim'_bisim. eapply bisim'_reduction_closed_1; eauto.
     eapply (S_star2 _ _ H0). eapply star2_refl.
   - eapply bisim_bisim' in H4.
     eapply bisim'_activated in H4; eauto.
     destruct H4 as [? [? [? []]]].
     destruct evt.
-    + eapply produces_prefix_star2_silent; eauto.
+    + eapply prefix_star2_silent; eauto.
       edestruct H6; eauto. destruct H8.
       econstructor 2. eauto. eapply H8.
-      eapply IHproduces_prefix; eauto.
+      eapply IHprefix; eauto.
       eapply bisim'_bisim. eapply H9.
     + exfalso; eapply (no_activated_tau_step _ H0 H1); eauto.
   - eapply bisim_bisim' in H4. eapply bisim'_terminate in H4; eauto.
@@ -99,7 +99,7 @@ Proof.
 Qed.
 
 Lemma bisim_prefix_eq {S} `{StateType S} {S'} `{StateType S'} (sigma:S) (σ':S')
-  : bisim sigma σ' -> forall L, produces_prefix sigma L <-> produces_prefix σ' L.
+  : bisim sigma σ' -> forall L, prefix sigma L <-> prefix σ' L.
 Proof.
   split; eapply bisim_prefix; eauto.
   eapply bisim_sym; eauto.
@@ -177,7 +177,7 @@ CoInductive coproduces {S} `{StateType S} : S -> stream extevent -> Prop :=
       -> activated σ'
       -> step σ' evt σ''
       -> coproduces σ'' L
-      -> coproduces σ (sons (EEvt evt) L)
+      -> coproduces σ (sons (EEvtExtern evt) L)
 | CoProducesSilent (σ:S) :
     diverges σ
     -> coproduces σ sil
@@ -185,7 +185,7 @@ CoInductive coproduces {S} `{StateType S} : S -> stream extevent -> Prop :=
   : result σ' = r
     -> star2 step σ nil σ'
     -> normal2 step σ'
-    -> coproduces σ (sons (EvtTerminate r) sil).
+    -> coproduces σ (sons (EEvtTerminate r) sil).
 
 Lemma coproduces_reduction_closed_step S `{StateType S} (σ σ':S) L
 : coproduces σ L -> step σ EvtTau σ'  -> coproduces σ' L.
@@ -232,7 +232,7 @@ Proof.
 Qed.
 
 Lemma produces_only_nil_diverges S `{StateType S} (σ:S)
-: (forall L, produces_prefix σ L -> L = nil) -> diverges σ.
+: (forall L, prefix σ L -> L = nil) -> diverges σ.
 Proof.
   revert σ. cofix f; intros.
   destruct (@step_dec _ H σ).
@@ -242,49 +242,49 @@ Proof.
       econstructor 4. congruence.
     + econstructor. eauto. eapply f.
       intros. eapply H0.
-      eapply produces_prefix_star2_silent.
+      eapply prefix_star2_silent.
       eapply (S_star2 EvtTau); eauto. econstructor. eauto.
   - exfalso.
     exploit H0. econstructor 3. reflexivity. econstructor. eauto. congruence.
 Qed.
 
-Lemma produces_prefix_extevent S `{StateType S} (σ:S) evt L
-: produces_prefix σ (EEvt evt::L)
+Lemma prefix_extevent S `{StateType S} (σ:S) evt L
+: prefix σ (EEvtExtern evt::L)
   -> exists σ', star2 step σ nil σ'
           /\ activated σ'
-          /\ exists σ'', step σ' evt σ'' /\ produces_prefix σ'' L.
+          /\ exists σ'', step σ' evt σ'' /\ prefix σ'' L.
 Proof.
   intros. general induction H0.
-  - edestruct IHproduces_prefix. reflexivity. dcr.
+  - edestruct IHprefix. reflexivity. dcr.
     eexists x; intuition. eapply (S_star2 EvtTau); eauto.
     eexists; eauto.
   - eexists σ; intuition. econstructor. eexists; eauto.
 Qed.
 
-Lemma produces_prefix_terminates S `{StateType S} (σ:S) r L
-:  produces_prefix σ (EvtTerminate r::L)
+Lemma prefix_terminates S `{StateType S} (σ:S) r L
+:  prefix σ (EEvtTerminate r::L)
    -> exists σ', star2 step σ nil σ' /\ normal2 step σ' /\ result σ' = r /\ L = nil.
 Proof.
   intros. general induction H0.
-  - edestruct IHproduces_prefix. reflexivity.
+  - edestruct IHprefix. reflexivity.
     eexists x; dcr; intuition. eapply (S_star2 EvtTau); eauto.
   - eexists; intuition; eauto.
 Qed.
 
 Lemma diverges_produces_only_nil S `{StateType S} S' `{StateType S'} (σ:S)
-: diverges σ -> (forall L, produces_prefix σ L -> L = nil).
+: diverges σ -> (forall L, prefix σ L -> L = nil).
 Proof.
   intros. general induction L; eauto.
   destruct a.
-  - eapply produces_prefix_extevent in H2; dcr.
+  - eapply prefix_extevent in H2; dcr.
     exfalso. eapply diverges_never_activated; eauto.
     eapply diverges_reduction_closed; eauto.
-  - eapply produces_prefix_terminates in H2; dcr; subst.
+  - eapply prefix_terminates in H2; dcr; subst.
     exfalso. eapply diverges_never_terminates; eauto using diverges_reduction_closed.
 Qed.
 
 Lemma produces_diverges S `{StateType S} S' `{StateType S'} (σ:S) (σ':S')
-: (forall L, produces_prefix σ L <-> produces_prefix σ' L)
+: (forall L, prefix σ L <-> prefix σ' L)
   -> diverges σ -> diverges σ'.
 Proof.
   revert σ σ'.
@@ -301,10 +301,10 @@ Proof.
   - econstructor. eapply H7.
     eapply f; intros; try eapply H4.
     split; intros.
-    + eapply produces_prefix_star2_silent'.
+    + eapply prefix_star2_silent'.
       eapply (S_star2 EvtTau). eapply H7. econstructor.
       eapply H1. econstructor; eauto.
-    + eapply produces_prefix_star2_silent'.
+    + eapply prefix_star2_silent'.
       eapply (S_star2 EvtTau). eapply H3. econstructor.
       eapply H1. econstructor; eauto.
   - exfalso.
@@ -313,12 +313,12 @@ Proof.
     congruence.
 Qed.
 
-Lemma produces_prefix_star_activated S `{StateType S} (σ1 σ1' σ1'':S) evt L
+Lemma prefix_star_activated S `{StateType S} (σ1 σ1' σ1'':S) evt L
 : star2 step σ1 nil σ1'
   -> activated σ1'
   -> step σ1' evt σ1''
-  -> produces_prefix σ1'' L
-  -> produces_prefix σ1 (EEvt evt::L).
+  -> prefix σ1'' L
+  -> prefix σ1 (EEvtExtern evt::L).
 Proof.
   intros. general induction H0.
   - econstructor 2; eauto.
@@ -326,60 +326,60 @@ Proof.
     econstructor; eauto.
 Qed.
 
-Lemma produces_prefix_preserved' S `{StateType S} S' `{StateType S'} (σ1 σ1' σ1'':S) (σ2 σ2' σ2'':S') evt
-: (forall L : list extevent, produces_prefix σ1 L <-> produces_prefix σ2 L)
+Lemma prefix_preserved' S `{StateType S} S' `{StateType S'} (σ1 σ1' σ1'':S) (σ2 σ2' σ2'':S') evt
+: (forall L : list extevent, prefix σ1 L <-> prefix σ2 L)
   -> star2 step σ1 nil σ1'
   -> activated σ1'
   -> step σ1' evt σ1''
   -> star2 step σ2 nil σ2'
   -> activated σ2'
   -> step σ2' evt σ2''
-  -> forall L, produces_prefix σ1'' L -> produces_prefix σ2'' L.
+  -> forall L, prefix σ1'' L -> prefix σ2'' L.
 Proof.
   intros.
-  - exploit (produces_prefix_star_activated _ H2 H3 H4 H8).
+  - exploit (prefix_star_activated _ H2 H3 H4 H8).
     eapply H1 in X.
-    eapply produces_prefix_extevent in X. dcr.
+    eapply prefix_extevent in X. dcr.
     exploit both_activated. eapply H10. eapply H5. eauto. eauto. subst.
     assert (x0 = σ2''). eapply step_externally_determined; eauto. subst; eauto.
 Qed.
 
 
-Lemma produces_prefix_preserved S `{StateType S} S' `{StateType S'} (σ1 σ1' σ1'':S) (σ2 σ2' σ2'':S') evt
+Lemma prefix_preserved S `{StateType S} S' `{StateType S'} (σ1 σ1' σ1'':S) (σ2 σ2' σ2'':S') evt
 :
-  (forall L : list extevent, produces_prefix σ1 L <-> produces_prefix σ2 L)
+  (forall L : list extevent, prefix σ1 L <-> prefix σ2 L)
   -> star2 step σ1 nil σ1'
   -> activated σ1'
   -> step σ1' evt σ1''
   -> star2 step σ2 nil σ2'
   -> activated σ2'
   -> step σ2' evt σ2''
-  -> forall L, produces_prefix σ1'' L <-> produces_prefix σ2'' L.
+  -> forall L, prefix σ1'' L <-> prefix σ2'' L.
 Proof.
   split; intros.
-  eapply (produces_prefix_preserved' _ _ H1); eauto.
+  eapply (prefix_preserved' _ _ H1); eauto.
   symmetry in H1.
-  eapply (produces_prefix_preserved' _ _ H1); eauto.
+  eapply (prefix_preserved' _ _ H1); eauto.
 Qed.
 
 Lemma produces_coproduces S `{StateType S} S' `{StateType S'} (σ:S) (σ':S')
-: (forall L, produces_prefix σ L <-> produces_prefix σ' L)
+: (forall L, prefix σ L <-> prefix σ' L)
   -> (forall T, coproduces σ T -> coproduces σ' T).
 Proof.
   revert σ σ'.
   cofix f; intros.
   inv H2.
-  - assert (produces_prefix σ (EEvt evt::nil)).
-    eapply produces_prefix_star_activated; eauto. econstructor 4.
+  - assert (prefix σ (EEvtExtern evt::nil)).
+    eapply prefix_star_activated; eauto. econstructor 4.
     eapply H1 in H7.
-    eapply produces_prefix_extevent in H7. dcr.
+    eapply prefix_extevent in H7. dcr.
     econstructor. eauto. eauto. eauto. eapply f; try eapply H6.
-    eapply (produces_prefix_preserved _ _ _ H1); eauto.
+    eapply (prefix_preserved _ _ _ H1); eauto.
   - exploit (produces_diverges H1 H3).
     econstructor. eauto.
-  - assert (produces_prefix σ (EvtTerminate (result σ'0)::nil)).
+  - assert (prefix σ (EEvtTerminate (result σ'0)::nil)).
     econstructor 3; eauto. eapply H1 in H3.
-    eapply produces_prefix_terminates in H3. dcr.
+    eapply prefix_terminates in H3. dcr.
     econstructor 3; eauto.
 Qed.
 
@@ -406,36 +406,36 @@ Qed.
 Lemma produces_silent_closed {S} `{StateType S}  S' `{StateType S'}  (σ1 σ1':S) (σ2 σ2':S')
 : star2 step σ1 nil σ1'
   -> star2 step σ2 nil σ2'
-  -> (forall L, produces_prefix σ1 L <-> produces_prefix σ2 L)
-  -> (forall L, produces_prefix σ1' L <-> produces_prefix σ2' L).
+  -> (forall L, prefix σ1 L <-> prefix σ2 L)
+  -> (forall L, prefix σ1' L <-> prefix σ2' L).
 Proof.
   split; intros.
-  - eapply produces_prefix_star2_silent'; eauto. eapply H3.
-    eapply produces_prefix_star2_silent; eauto.
-  - eapply produces_prefix_star2_silent'; eauto. eapply H3.
-    eapply produces_prefix_star2_silent; eauto.
+  - eapply prefix_star2_silent'; eauto. eapply H3.
+    eapply prefix_star2_silent; eauto.
+  - eapply prefix_star2_silent'; eauto. eapply H3.
+    eapply prefix_star2_silent; eauto.
 Qed.
 
-Lemma produces_prefix_bisim S `{StateType S} S' `{StateType S'} (σ:S) (σ':S')
-: (forall L, produces_prefix σ L <-> produces_prefix σ' L)
+Lemma prefix_bisim S `{StateType S} S' `{StateType S'} (σ:S) (σ':S')
+: (forall L, prefix σ L <-> prefix σ' L)
   -> bisim σ σ'.
 Proof.
   revert σ σ'.
   cofix f; intros.
   destruct (three_possibilities σ) as [A|[A|A]].
-  - dcr. assert (produces_prefix σ (EvtTerminate (result x)::nil)).
+  - dcr. assert (prefix σ (EEvtTerminate (result x)::nil)).
     econstructor 3; eauto.
     eapply H1 in H2.
-    eapply produces_prefix_terminates in H2. dcr.
+    eapply prefix_terminates in H2. dcr.
     econstructor 3; eauto.
   - dcr. inv H4; dcr.
-    assert (produces_prefix x1 nil) by econstructor 4.
-    exploit (produces_prefix_star_activated _ H3 H4 H5 H2).
+    assert (prefix x1 nil) by econstructor 4.
+    exploit (prefix_star_activated _ H3 H4 H5 H2).
     eapply H1 in X.
-    eapply produces_prefix_extevent in X. dcr.
+    eapply prefix_extevent in X. dcr.
     econstructor 2; eauto.
     + intros.
-      assert (B:produces_prefix x (EEvt evt::nil)) by
+      assert (B:prefix x (EEvtExtern evt::nil)) by
           (econstructor 2; eauto; econstructor 4).
       pose proof H1.
       eapply produces_silent_closed in H11; eauto.
@@ -443,9 +443,9 @@ Proof.
       inv B.
       * exfalso. exploit (step_internally_deterministic _ _ _ _ H12 H9 ); eauto. dcr; congruence.
       * eexists; split. eauto. eapply f.
-        eapply produces_prefix_preserved; eauto.
+        eapply prefix_preserved; eauto.
     + intros.
-      assert (B:produces_prefix x2 (EEvt evt::nil)) by
+      assert (B:prefix x2 (EEvtExtern evt::nil)) by
           (econstructor 2; eauto; econstructor 4).
       pose proof H1.
       eapply produces_silent_closed in H11; eauto.
@@ -453,7 +453,7 @@ Proof.
       inv B.
       * exfalso. exploit (step_internally_deterministic _ _ _ _ H12 H5 ); eauto. dcr; congruence.
       * eexists; split. eauto. eapply f.
-        eapply produces_prefix_preserved; eauto.
+        eapply prefix_preserved; eauto.
   - assert (diverges σ').
     eapply (produces_diverges H1); eauto.
     eapply bisim_complete_diverges; eauto.
