Equiv/TraceApx.v
@@ -1,0 +1,1022 @@
+Require Import List.
+Require Export Util Var Val Exp Env Map CSet AutoIndTac IL AllInRel.
+Require Export EventsActivated StateType paco Equiv Bisim Sim.
+
+Set Implicit Arguments.
+Unset Printing Records.
+
+Inductive extevent :=
+  | EEvtExtern (ext:extern)
+  | EEvtTerminate (res:val).
+
+Inductive produces_prefix {S} `{StateType S} : S -> list extevent -> Prop :=
+  | producesPrefixSilent (σ:S) (σ':S) L :
+      step σ EvtTau σ'
+      -> produces_prefix σ' L
+      -> produces_prefix σ  L
+  | producesPrefixExtern (σ:S) (σ':S) ext L :
+      activated σ
+      -> step σ (EvtExtern ext) σ'
+      -> produces_prefix σ' L
+      -> produces_prefix σ (EEvtExtern ext::L)
+  | producesPrefixTerm (σ:S) (σ':S) r
+    : result σ' = Some r
+      -> star2 step σ nil σ'
+      -> normal2 step σ'
+      -> produces_prefix σ (EEvtTerminate r::nil)
+  | producesPrefixCrash (σ:S) (σ':S) L
+    : result σ' = None
+      -> star2 step σ nil σ'
+      -> normal2 step σ'
+      -> produces_prefix σ L
+  | producesPrefixPrefix (σ:S)
+    : produces_prefix σ nil.
+
+Lemma produces_prefix_star2_silent {S} `{StateType S} (σ σ':S) L
+ : star2 step σ nil σ' ->
+   produces_prefix σ' L -> produces_prefix σ L.
+Proof.
+  intros. general induction H0; eauto.
+  - destruct yl, y; simpl in *; try congruence.
+    econstructor 1; eauto.
+Qed.
+
+Lemma star2_reach_silent_step (X : Type) (R:X -> event -> X -> Prop) (x y z : X)
+: R x EvtTau y
+  -> star2 R x nil z
+  -> internally_deterministic R
+  -> x = z \/ star2 R y nil z.
+Proof.
+  intros. inv H0; eauto.
+  exploit H1; eauto. dcr; subst; eauto.
+Qed.
+
+
+Lemma produces_prefix_star2_silent' {S} `{StateType S} (σ σ':S) L
+ : star2 step σ nil σ' ->
+   produces_prefix σ L -> produces_prefix σ' L.
+Proof.
+  intros. general induction H0; eauto.
+  - destruct yl, y; simpl in *; try congruence.
+    eapply IHstar2; eauto.
+    inv H2.
+    + exploit step_internally_deterministic. eapply H. eapply H3.
+      dcr; subst. eauto.
+    + exfalso. inv H3; dcr.
+      exploit step_internally_deterministic. eapply H. eapply H7. dcr; congruence.
+    + exploit star2_reach_silent_step; eauto. eapply H1.
+      destruct X; subst. exfalso. eapply H5; firstorder.
+      econstructor 3; eauto.
+    + exploit star2_reach_silent_step; eauto. eapply H1.
+      destruct X; subst. exfalso. eapply H5; firstorder.
+      econstructor 4; eauto.
+    + econstructor 5; eauto.
+Qed.
+
+Lemma no_activated_tau_step {S} `{StateType S} (σ σ':S)
+ :  activated σ
+  -> step σ EvtTau σ'
+  -> False.
+Proof.
+  intros. destruct H0 as [? [? ?]].
+  eapply step_internally_deterministic in H0; eauto.
+  dcr; congruence.
+Qed.
+
+Lemma bisim_prefix {S} `{StateType S} {S'} `{StateType S'} (sigma:S) (σ':S')
+: bisim sigma σ' -> forall L, produces_prefix sigma L -> produces_prefix σ' L.
+Proof.
+  intros. general induction H2.
+  - eapply bisim_bisim' in H3.
+    eapply IHproduces_prefix; eauto.
+    eapply bisim'_bisim. eapply bisim'_reduction_closed_1; eauto.
+    eapply (S_star2 _ _ H0). eapply star2_refl.
+  - eapply bisim_bisim' in H4.
+    eapply bisim'_activated in H4; eauto.
+    destruct H4 as [? [? [? []]]].
+    + eapply produces_prefix_star2_silent; eauto.
+      edestruct H6; eauto. destruct H8.
+      econstructor 2. eauto. eapply H8.
+      eapply IHproduces_prefix; eauto.
+      eapply bisim'_bisim. eapply H9.
+  - eapply bisim_bisim' in H4. eapply bisim'_terminate in H4; eauto.
+    destruct H4 as [? [? []]].
+    econstructor 3; [ | eauto | eauto]. congruence.
+  - eapply bisim_bisim' in H4. eapply bisim'_terminate in H4; eauto.
+    destruct H4 as [? [? []]]. econstructor 4; [ | eauto | eauto]. congruence.
+  - econstructor 5; eauto.
+Qed.
+
+Lemma bisim_prefix_eq {S} `{StateType S} {S'} `{StateType S'} (sigma:S) (σ':S')
+  : bisim sigma σ' -> forall L, produces_prefix sigma L <-> produces_prefix σ' L.
+Proof.
+  split; eapply bisim_prefix; eauto.
+  eapply bisim_sym; eauto.
+Qed.
+
+CoInductive diverges S `{StateType S} : S -> Prop :=
+| DivergesI σ σ'
+  : step σ EvtTau σ'
+    -> diverges σ'
+    -> diverges σ.
+
+Lemma diverges_reduction_closed S `{StateType S} (σ σ':S)
+: diverges σ -> star2 step σ nil σ'  -> diverges σ'.
+Proof.
+  intros. general induction H1; eauto using diverges.
+  destruct yl, y; simpl in *; try congruence.
+  inv H2.
+  exploit step_internally_deterministic.
+  eapply H. eapply H3. dcr; subst.
+  eapply IHstar2; eauto.
+Qed.
+
+Lemma diverges_never_activated S `{StateType S} (σ:S)
+: activated σ -> diverges σ -> False.
+Proof.
+  intros. inv H0. inv H1. dcr.
+  exploit step_internally_deterministic.
+  eapply H3. eapply H5. dcr; congruence.
+Qed.
+
+Lemma diverges_never_terminates S `{StateType S} (σ σ':S) A
+: normal2 step σ' -> star2 step σ A σ' -> diverges σ -> False.
+Proof.
+  intros. general induction H1.
+  - inv H2. firstorder.
+  - inv H3.
+    exploit (step_internally_deterministic). eauto. eapply H. dcr; subst.
+    eapply IHstar2; eauto.
+Qed.
+
+Definition crashes S `{StateType S} (σ:S) :=
+  exists σ', star2 step σ nil σ' /\ normal2 step σ' /\ result σ' = None.
+
+Lemma diverges_never_crashes S `{StateType S} (σ σ':S)
+: crashes σ -> diverges σ -> False.
+Proof.
+  intros. destruct H0; dcr.
+  eapply diverges_never_terminates; eauto.
+Qed.
+
+Lemma crashes_not_activated S `{StateType S} (σ σ':S)
+: crashes σ -> star2 step σ nil σ' -> activated σ' -> False.
+Proof.
+  intros. destruct H0. dcr.
+  eauto using activated_normal_star.
+Qed.
+
+Lemma bisim_sound_diverges S `{StateType S} S' `{StateType S'} (σ:S) (σ':S')
+: bisim σ σ' -> diverges σ -> diverges σ'.
+Proof.
+  revert σ σ'. cofix COH; intros.
+  inv H1.
+  - eapply plus2_destr_nil in H4. dcr.
+    econstructor. eauto.
+    eapply COH; eauto.
+    eapply bisim'_bisim.
+    eapply bisim'_reduction_closed.
+    eapply bisim_bisim'. eapply H1. econstructor.
+    eapply (S_star2 EvtTau); eauto. econstructor.
+  - eapply diverges_reduction_closed in H3.
+    + exfalso. eapply (diverges_never_activated H5); eauto.
+    + eapply H2.
+  - eapply diverges_reduction_closed in H4.
+    + exfalso. eapply (diverges_never_terminates H6); eauto. constructor.
+    + eapply H2.
+Qed.
+
+Lemma bisim_complete_diverges S `{StateType S} S' `{StateType S'} (σ:S) (σ':S')
+: diverges σ -> diverges σ' -> bisim σ σ'.
+Proof.
+  revert σ σ'. cofix COH; intros.
+  inv H1; inv H2.
+  econstructor. econstructor; eauto. econstructor; eauto.
+  eapply COH; eauto.
+Qed.
+
+
+Lemma sim_sound_diverges S `{StateType S} S' `{StateType S'} (σ:S) (σ':S')
+: sim σ σ' -> diverges σ -> diverges σ'.
+Proof.
+  revert σ σ'. cofix COH; intros.
+  inv H1.
+  - eapply plus2_destr_nil in H4. dcr.
+    econstructor. eauto.
+    eapply COH; eauto.
+    eapply sim'_sim.
+    eapply sim'_reduction_closed.
+    eapply sim_sim'. eapply H1. econstructor.
+    eapply (S_star2 EvtTau); eauto. econstructor.
+  - eapply diverges_reduction_closed in H3.
+    + exfalso. eapply (diverges_never_activated H5); eauto.
+    + eapply H2.
+  - eapply diverges_reduction_closed in H4.
+    + exfalso. eapply (diverges_never_terminates H5); eauto. constructor.
+    + eapply H2.
+  - eapply diverges_reduction_closed in H4.
+    + exfalso. eapply (diverges_never_terminates H6); eauto. constructor.
+    + eapply H2.
+Qed.
+
+Lemma sim_complete_diverges S `{StateType S} S' `{StateType S'} (σ:S) (σ':S')
+: diverges σ -> diverges σ' -> sim σ σ'.
+Proof.
+  revert σ σ'. cofix COH; intros.
+  inv H1; inv H2.
+  econstructor. econstructor; eauto. econstructor; eauto.
+  eapply COH; eauto.
+Qed.
+
+CoInductive stream (A : Type) : Type :=
+| sil : stream A
+| sons : A -> stream A -> stream A.
+
+Arguments sil [A].
+
+(*
+CoInductive coproduces {S} `{StateType S} : S -> stream extevent -> Prop :=
+| CoProducesExtern (σ σ' σ'':S) ext L :
+    star2 step σ nil σ'
+      -> activated σ'
+      -> step σ' (EvtExtern ext) σ''
+      -> coproduces σ'' L
+      -> coproduces σ (sons (EEvt ext) L)
+| CoProducesSilent (σ:S) :
+    diverges σ
+    -> coproduces σ sil
+| CoProducesTerm (σ:S) (σ':S) r
+  : result σ' = r
+    -> star2 step σ nil σ'
+    -> normal2 step σ'
+    -> coproduces σ (sons (EvtTerminate r) sil).
+
+Lemma coproduces_reduction_closed_step S `{StateType S} (σ σ':S) L
+: coproduces σ L -> step σ EvtTau σ'  -> coproduces σ' L.
+Proof.
+  intros. inv H0.
+  - exploit activated_star_reach. eapply H3. eauto.
+    eapply (S_star2 EvtTau); eauto. econstructor.
+    econstructor. eapply X. eauto. eauto. eauto.
+  - econstructor. eapply diverges_reduction_closed; eauto.
+    eapply (S_star2 EvtTau); eauto. econstructor.
+  - exploit star2_reach_normal. eauto.
+    eapply (S_star2 EvtTau); eauto. econstructor.
+    eapply H. eauto.
+    econstructor; try eapply X. eauto. eauto.
+Qed.
+
+Lemma coproduces_reduction_closed S `{StateType S} (σ σ':S) L
+: coproduces σ L -> star2 step σ nil σ'  -> coproduces σ' L.
+Proof.
+  intros. general induction H1; eauto using coproduces. eauto.
+  destruct yl, y; simpl in *; try congruence.
+  eapply IHstar2; eauto.
+  eapply coproduces_reduction_closed_step; eauto.
+Qed.
+
+Lemma bisim_coproduces S `{StateType S} S' `{StateType S'} (sigma:S) (σ':S')
+  : bisim sigma σ' -> forall L, coproduces sigma L -> coproduces σ' L.
+Proof.
+  revert sigma σ'. cofix COH; intros.
+  inv H2.
+  - assert (bisim' σ'0 σ').
+    eapply bisim'_reduction_closed. eapply (bisim_bisim' H1).
+    eauto. econstructor.
+    exploit (bisim'_activated H4 H7). dcr.
+    edestruct H10. eauto. dcr.
+    econstructor; try eapply H8. eauto. eapply H11.
+    eapply COH; eauto.
+    destruct H11.
+    eapply bisim'_bisim. eapply H13.
+  - econstructor. eapply (bisim_sound_diverges H1); eauto.
+  - exploit (bisim'_terminate H4 H5 (bisim_bisim' H1)).
+    dcr.
+    econstructor; eauto.
+Qed.
+ *)
+
+Lemma produces_prefix_extevent S `{StateType S} (σ:S) evt L
+: produces_prefix σ (EEvtExtern evt::L)
+  -> ~ crashes σ
+  -> exists σ', star2 step σ nil σ'
+          /\ activated σ'
+          /\ exists σ'', step σ' (EvtExtern evt) σ'' /\ produces_prefix σ'' L.
+Proof.
+  intros. general induction H0.
+  - edestruct IHproduces_prefix. reflexivity.
+    + intro. eapply H2. inv H3; dcr.
+      eexists; split; eauto. eapply (S_star2 EvtTau); eauto.
+    + eexists x; intuition. eapply (S_star2 EvtTau); eauto.
+  - eexists σ; intuition. econstructor. eexists; eauto.
+  - exfalso. eapply H3. eexists; eauto.
+Qed.
+
+Lemma produces_prefix_terminates S `{StateType S} (σ:S) r L
+:  produces_prefix σ (EEvtTerminate r::L)
+   -> ~ crashes σ
+   -> exists σ', star2 step σ nil σ' /\ normal2 step σ' /\ result σ' = Some r /\ L = nil.
+Proof.
+  intros. general induction H0.
+  - edestruct IHproduces_prefix. reflexivity.
+    + intro. eapply H2. inv H3; dcr.
+      eexists; split; eauto. eapply (S_star2 EvtTau); eauto.
+    + eexists x; dcr; intuition. eapply (S_star2 EvtTau); eauto.
+  - eexists; intuition; eauto.
+  - exfalso; eapply H3.
+    eexists; eauto.
+Qed.
+
+Lemma diverges_produces_only_nil S `{StateType S} S' `{StateType S'} (σ:S)
+: diverges σ -> (forall L, produces_prefix σ L -> L = nil).
+Proof.
+  intros. general induction L; eauto.
+  destruct a.
+  - eapply produces_prefix_extevent in H2; dcr.
+    exfalso. eapply diverges_never_activated; eauto.
+    eapply diverges_reduction_closed; eauto.
+    intro. eapply diverges_never_crashes; eauto.
+  - eapply produces_prefix_terminates in H2; dcr; subst.
+    exfalso. eapply diverges_never_terminates; eauto using diverges_reduction_closed.
+    eauto using diverges_never_crashes.
+Qed.
+
+Lemma produces_only_nil_diverges S `{StateType S} (σ:S)
+: (forall L, produces_prefix σ L -> L = nil) -> diverges σ.
+Proof.
+  revert σ. cofix f; intros.
+  destruct (@step_dec _ H σ).
+  - destruct H1; dcr. destruct x.
+    + exfalso. exploit H0. econstructor 2; try eapply H2.
+      eexists; eauto.
+      econstructor 5. congruence.
+    + econstructor. eauto. eapply f.
+      intros. eapply H0.
+      eapply produces_prefix_star2_silent.
+      eapply (S_star2 EvtTau); eauto. econstructor. eauto.
+  - exfalso. case_eq (result σ); intros.
+    + exploit H0. econstructor 3; eauto. constructor. congruence.
+    + exploit H0. econstructor 4; eauto. constructor.
+      instantiate (1:=EEvtExtern (ExternI 0 nil 0)::nil) in X.
+      congruence.
+Qed.
+
+Lemma produces_diverges' S `{StateType S} S' `{StateType S'} (σ:S) (σ':S')
+: (forall L, produces_prefix σ' L -> produces_prefix σ L)
+  -> diverges σ -> diverges σ'.
+Proof.
+  revert σ σ'.
+  cofix f; intros.
+  inv H2.
+  edestruct (@step_dec _ H0 σ').
+  inv H5; dcr.
+  destruct x.
+  - exfalso.
+    pose proof (diverges_produces_only_nil H2).
+    exploit H6. eapply H1.
+    econstructor 2. eexists; eauto. eauto. econstructor 5.
+    congruence.
+  - econstructor. eapply H7.
+    eapply f; intros; try eapply H4.
+    + eapply produces_prefix_star2_silent'.
+      eapply (S_star2 EvtTau). eapply H3. econstructor.
+      eapply H1. econstructor; eauto.
+  - exfalso.
+    case_eq (result σ'); intros.
+    + exploit (diverges_produces_only_nil H2).
+      eapply H1. econstructor 3; eauto. constructor.
+      congruence.
+    + exploit (diverges_produces_only_nil H2).
+      eapply H1. econstructor 4; eauto. constructor.
+      instantiate (1:=EEvtExtern (ExternI 0 nil 0)::nil) in X.
+      congruence.
+Qed.
+
+Lemma produces_diverges S `{StateType S} S' `{StateType S'} (σ:S) (σ':S')
+: (forall L, produces_prefix σ L <-> produces_prefix σ' L)
+  -> diverges σ -> diverges σ'.
+Proof.
+  intros.
+  eapply (@produces_diverges' S _ S' _); eauto.
+  eapply H1; eauto.
+Qed.
+
+
+Lemma produces_prefix_star_activated S `{StateType S} (σ1 σ1' σ1'':S) ext L
+: star2 step σ1 nil σ1'
+  -> activated σ1'
+  -> step σ1' (EvtExtern ext) σ1''
+  -> produces_prefix σ1'' L
+  -> produces_prefix σ1 (EEvtExtern ext::L).
+Proof.
+  intros. general induction H0.
+  - econstructor 2; eauto.
+  - destruct y, yl; simpl in *; try congruence.
+    econstructor; eauto.
+Qed.
+
+Lemma produces_prefix_preserved' S `{StateType S} S' `{StateType S'} (P : list extevent -> Prop)
+      (PEXT:forall L e, P L -> P (EEvtExtern e::L))
+      (σ1 σ1' σ1'':S) (σ2 σ2' σ2'':S') ext
+: (forall L : list extevent, P L -> produces_prefix σ1 L -> produces_prefix σ2 L)
+  -> star2 step σ1 nil σ1'
+  -> activated σ1'
+  -> step σ1' (EvtExtern ext) σ1''
+  -> star2 step σ2 nil σ2'
+  -> activated σ2'
+  -> step σ2' (EvtExtern ext) σ2''
+  -> forall L, P L -> produces_prefix σ1'' L -> produces_prefix σ2'' L.
+Proof.
+  intros.
+  - exploit (produces_prefix_star_activated _ H2 H3 H4 H9).
+    eapply H1 in X.
+    eapply produces_prefix_extevent in X. dcr.
+    exploit both_activated. eapply H11. eapply H5. eauto. eauto. subst.
+    assert (x0 = σ2''). eapply step_externally_determined; eauto. subst; eauto.
+    eauto using crashes_not_activated.
+    eauto using no_activated_tau_step.
+Qed.
+
+Lemma produces_prefix_preserved S `{StateType S} S' `{StateType S'}
+      (P : list extevent -> Prop)
+      (PEXT:forall L e, P L -> P (EEvtExtern e::L))
+      (σ1 σ1' σ1'':S) (σ2 σ2' σ2'':S') ext
+:
+  (forall L : list extevent, P L -> (produces_prefix σ1 L <-> produces_prefix σ2 L))
+  -> star2 step σ1 nil σ1'
+  -> activated σ1'
+  -> step σ1' (EvtExtern ext) σ1''
+  -> star2 step σ2 nil σ2'
+  -> activated σ2'
+  -> step σ2' (EvtExtern ext) σ2''
+  -> forall L, P L -> (produces_prefix σ1'' L <-> produces_prefix σ2'' L).
+Proof.
+  split; intros.
+  eapply (@produces_prefix_preserved' S _ S' _ P); intros; eauto.
+  eapply H1; eauto.
+  eapply (@produces_prefix_preserved' S' _ S _ P); intros; eauto.
+  eapply H1; eauto.
+Qed.
+
+(*
+Lemma produces_coproduces S `{StateType S} S' `{StateType S'} (σ:S) (σ':S')
+: (forall L, produces_prefix σ L <-> produces_prefix σ' L)
+  -> (forall T, coproduces σ T -> coproduces σ' T).
+Proof.
+  revert σ σ'.
+  cofix f; intros.
+  inv H2.
+  - assert (produces_prefix σ (EEvt ext::nil)).
+    eapply produces_prefix_star_activated; eauto. econstructor 5.
+    eapply H1 in H7.
+    eapply produces_prefix_extevent in H7. dcr.
+    econstructor. eauto. eauto. eauto. eapply f; try eapply H6.
+    intros.
+    eapply (produces_prefix_preserved (fun _ => True)); eauto.
+    admit.
+  - eapply produces_diverges in H3.
+    econstructor; eauto. eauto.
+  - case_eq (result σ'0); intros.
+    + assert (produces_prefix σ (EvtTerminate (result σ'0)::nil)). {
+        + rewrite H3. econstructor 3; eauto.
+      }
+    eapply H1 in H6.
+    eapply produces_prefix_terminates in H6. dcr.
+    econstructor 3; eauto. rewrite H9; eauto.
+    intro. admit.
+    + admit.
+Admitted.
+ *)
+
+Require Import Classical_Prop.
+
+Lemma three_possibilities S `{StateType S} (σ:S)
+: (exists σ', star2 step σ nil σ' /\ normal2 step σ')
+  \/ (exists σ', star2 step σ nil σ' /\ activated σ')
+  \/ diverges σ.
+Proof.
+  destruct (classic (exists σ' : S, star2 step σ nil σ' /\ normal2 step σ')); intuition; right.
+  destruct (classic (exists σ' : S, star2 step σ nil σ' /\ activated σ')); intuition; right.
+  revert σ H0 H1. cofix f.
+  intros. destruct (@step_dec _ H σ). inv H2; dcr.
+  destruct x.
+  - exfalso. eapply H1; eexists σ; intuition.
+    econstructor. do 2 eexists; eauto.
+  - econstructor. eauto. eapply f; intros; dcr.
+    eapply H0; eexists; split; eauto. eapply (S_star2 EvtTau); eauto.
+    eapply H1; eexists; split; eauto. eapply (S_star2 EvtTau); eauto.
+  - exfalso. eapply H0; eexists σ; intuition. econstructor.
+Qed.
+
+Lemma produces_silent_closed {S} `{StateType S}  S' `{StateType S'}  (σ1 σ1':S) (σ2 σ2':S')
+: star2 step σ1 nil σ1'
+  -> star2 step σ2 nil σ2'
+  -> (forall L, produces_prefix σ1 L <-> produces_prefix σ2 L)
+  -> (forall L, produces_prefix σ1' L <-> produces_prefix σ2' L).
+Proof.
+  split; intros.
+  - eapply produces_prefix_star2_silent'; eauto. eapply H3.
+    eapply produces_prefix_star2_silent; eauto.
+  - eapply produces_prefix_star2_silent'; eauto. eapply H3.
+    eapply produces_prefix_star2_silent; eauto.
+Qed.
+
+Lemma terminates_not_crashes S `{StateType S} (σ:S) (σ':S) v
+:  star2 step σ nil σ'
+   -> normal2 step σ'
+   -> result σ' = ⎣ v ⎦
+   -> ~ crashes σ.
+Proof.
+  intros. intro. destruct H3; dcr.
+  assert (x = σ'). eapply star2_reach_normal2; eauto. eapply H.
+  subst. congruence.
+Qed.
+
+Lemma produces_all_prefixes_crashes S `{StateType S} S' `{StateType S'} (σ:S) (σ':S')
+: (forall L, produces_prefix σ L) <-> crashes σ.
+Proof.
+  split; intros.
+  - destruct (classic (crashes σ)); eauto.
+    exfalso.
+    assert (produces_prefix σ (EEvtExtern (ExternI 0 nil 0)::nil)) by eauto.
+    assert (produces_prefix σ (EEvtTerminate 0::nil)) by eauto.
+    exploit (produces_prefix_terminates H4); eauto.
+    exploit (produces_prefix_extevent H3); eauto. dcr.
+    exploit (star2_reach_normal H10 H6); eauto. eapply H.
+    eauto using @activated_normal_star.
+  - destruct H1 as [? [? []]].
+    econstructor 4; eauto.
+Qed.
+
+Lemma crashes_bisim S `{StateType S} S' `{StateType S'} (σ:S) (σ':S')
+:  crashes σ
+   -> crashes σ'
+   -> bisim σ σ'.
+Proof.
+  intros. destruct H1, H2; dcr.
+  econstructor 3; eauto. congruence.
+Qed.
+
+Lemma produces_prefix_bisim S `{StateType S} S' `{StateType S'} (σ:S) (σ':S')
+: (forall L, produces_prefix σ L <-> produces_prefix σ' L)
+  -> bisim σ σ'.
+Proof.
+  revert σ σ'.
+  cofix f; intros.
+  destruct (three_possibilities σ) as [A|[A|A]].
+  - dcr. case_eq (result x); intros.
+    + assert (produces_prefix σ (EEvtTerminate v::nil)).
+      econstructor 3; eauto.
+      eapply H1 in H5.
+      eapply produces_prefix_terminates in H5. dcr.
+      econstructor 3; eauto. congruence.
+      * intro. pose proof (terminates_not_crashes H3 H4 H2).
+        rewrite <- produces_all_prefixes_crashes in H6; eauto.
+        assert (forall L : list extevent, produces_prefix σ L). {
+          intros. eapply H1. eauto.
+        }
+        rewrite produces_all_prefixes_crashes in H8; eauto.
+    + clear f.
+      assert (crashes σ). eexists; split. eauto. eauto.
+      assert (crashes σ').
+      rewrite <- produces_all_prefixes_crashes in H5; [|eauto|eauto].
+      assert (forall L : list extevent, produces_prefix σ' L) by firstorder.
+      rewrite produces_all_prefixes_crashes in H6; [|eauto|eauto].
+      eauto.
+      eapply crashes_bisim; eauto. Guarded.
+  - dcr. inv H4; dcr.
+    assert (produces_prefix x1 nil) by econstructor 5.
+    exploit (produces_prefix_star_activated _ H3 H4 H5 H2).
+    eapply H1 in X.
+    eapply produces_prefix_extevent in X. dcr.
+    econstructor 2; eauto. Guarded.
+    + intros. destruct evt.
+      assert (B:produces_prefix x (EEvtExtern call::nil)).
+      econstructor 2. eauto. eauto. econstructor 5.
+      pose proof H1.
+      eapply produces_silent_closed in H11; eauto.
+      eapply H11 in B.
+      inv B.
+      * exfalso. exploit (step_internally_deterministic _ _ _ _ H12 H9 ); eauto. dcr; congruence.
+      * eexists; split. eauto. eapply f.
+        intros. Guarded.
+        eapply (produces_prefix_preserved (fun _ => True)); eauto.
+      * exfalso. eauto using activated_normal_star, star2.
+      * exfalso. exploit (step_internally_deterministic _ _ _ _ H8 H5 ); eauto. dcr; congruence.
+    + intros. destruct evt.
+      assert (B:produces_prefix x2 (EEvtExtern call::nil)).
+      econstructor 2. eauto. eauto. econstructor 5.
+      pose proof H1.
+      eapply produces_silent_closed in H11; eauto.
+      eapply H11 in B.
+      inv B.
+      * exfalso. exploit (step_internally_deterministic _ _ _ _ H12 H5 ); eauto. dcr; congruence.
+      * eexists; split. eauto. eapply f.
+        intros. Guarded.
+        eapply (produces_prefix_preserved (fun _ => True)); eauto.
+      * exfalso. eapply (activated_normal_star (star2_refl _ _) H4). eauto. eauto.
+      * exfalso. exploit (step_internally_deterministic _ _ _ _ H8 H9 ); eauto. dcr; congruence.
+    + clear f.
+      intro.
+      assert (crashes σ).
+      rewrite <- produces_all_prefixes_crashes in H6; [|eauto|eauto].
+      assert (forall L : list extevent, produces_prefix σ L) by firstorder.
+      rewrite produces_all_prefixes_crashes in H7; [|eauto|eauto].
+      eauto.
+      eapply (crashes_not_activated H7). eauto. eauto.
+  - assert (diverges σ').
+    eapply (produces_diverges H1); eauto.
+    eapply bisim_complete_diverges; eauto.
+Qed.
+
+Inductive not_crashed : list extevent -> Prop :=
+| NotCrashedTrm v
+  : not_crashed (EEvtTerminate v::nil)
+| NotCrashedDiv
+  : not_crashed nil
+| NotCrashedStep e es
+  : not_crashed es
+    -> not_crashed (EEvtExtern e::es).
+
+Lemma produces_not_crashed_silent_closed {S} `{StateType S}  S' `{StateType S'}  (σ1 σ1':S) (σ2 σ2':S')
+: star2 step σ1 nil σ1'
+  -> star2 step σ2 nil σ2'
+  -> (forall L, not_crashed L -> (produces_prefix σ1 L <-> produces_prefix σ2 L))
+  -> (forall L, not_crashed L -> (produces_prefix σ1' L <-> produces_prefix σ2' L)).
+Proof.
+    split; intros.
+  - eapply produces_prefix_star2_silent'; eauto. eapply H3. eauto.
+    eapply produces_prefix_star2_silent; eauto.
+  - eapply produces_prefix_star2_silent'; eauto. eapply H3. eauto.
+    eapply produces_prefix_star2_silent; eauto.
+Qed.
+
+Lemma produces_not_crashed_silent_closed' {S} `{StateType S}  S' `{StateType S'}  (σ1 σ1':S) (σ2 σ2':S')
+: star2 step σ1 nil σ1'
+  -> star2 step σ2 nil σ2'
+  -> (forall L, not_crashed L -> (produces_prefix σ1 L -> produces_prefix σ2 L))
+  -> (forall L, not_crashed L -> (produces_prefix σ1' L -> produces_prefix σ2' L)).
+Proof.
+  intros.
+  - eapply produces_prefix_star2_silent'; eauto. eapply H3. eauto.
+    eapply produces_prefix_star2_silent; eauto.
+Qed.
+
+CoInductive crashdiverges S `{StateType S} : S -> Prop :=
+| CrashDivergesDiv σ σ'
+  : step σ EvtTau σ'
+    -> crashdiverges σ'
+    -> crashdiverges σ
+| CrashDivergesCrash σ
+  : normal2 step σ
+    -> result σ = None
+    ->  crashdiverges σ.
+
+Lemma crashdiverges_not_diverges S `{StateType S} (σ:S)
+: ~ crashes σ -> crashdiverges σ -> diverges σ.
+Proof.
+  revert σ. cofix f. intros.
+  inv H1.
+  - econstructor; eauto. eapply f.
+    intro. eapply H0. destruct H4. dcr.
+    eexists x; repeat split; eauto. eapply (S_star2 EvtTau); eauto.
+    eauto.
+  - exfalso. eapply H0. eexists σ; split; eauto. econstructor.
+Qed.
+
+Lemma crashdiverges_crashes_or_diverges S `{StateType S} (σ:S)
+: crashdiverges σ -> crashes σ \/ diverges σ.
+Proof.
+  destruct (classic (crashes σ)); eauto using crashdiverges_not_diverges.
+Qed.
+
+Lemma crash_crashdiverges  S `{StateType S} (σ σ':S)
+: star2 step σ nil σ'
+  -> normal2 step σ'
+  -> result σ' = None
+  -> crashdiverges σ.
+Proof.
+  intros. general induction H0; eauto using crashdiverges.
+  destruct y,yl; simpl in *; try congruence.
+  eauto using crashdiverges.
+Qed.
+
+Lemma produces_not_crashed_prefix_sim S `{StateType S} S' `{StateType S'} (σ:S) (σ':S')
+: (forall L, produces_prefix σ' L -> produces_prefix σ L)
+  -> sim σ σ'.
+Proof.
+  revert σ σ'.
+  cofix f; intros.
+  destruct (classic (crashes σ)).
+  clear f. inv H2. econstructor 3. eapply H3. eauto. eapply H3.
+  destruct (three_possibilities σ') as [A|[A|A]].
+  - dcr. case_eq (result x); intros.
+    + assert (produces_prefix σ' (EEvtTerminate v::nil)).
+      econstructor 3; eauto.
+      eapply H1 in H6.
+      eapply produces_prefix_terminates in H6. dcr.
+      econstructor 4; eauto. congruence. eauto.
+    + clear f. exfalso.
+      assert (crashes σ'). eexists; split. eauto. eauto.
+      eapply H2.
+      rewrite <- produces_all_prefixes_crashes in H6; [|eauto|eauto].
+      assert (forall L : list extevent, produces_prefix σ L) by firstorder.
+      rewrite produces_all_prefixes_crashes in H7; [|eauto|eauto].
+      eauto.
+  - dcr. inv H5; dcr.
+    assert (produces_prefix x1 nil) by econstructor 5.
+    exploit (produces_prefix_star_activated _ H4 H5 H6 H3).
+    eapply H1 in X.
+    eapply produces_prefix_extevent in X. dcr.
+    econstructor 2; eauto. Guarded.
+    + (* intros. destruct evt.
+      assert (B:produces_prefix x2 (EEvtExtern call::nil)).
+      econstructor 2. eauto. eauto. econstructor 5.
+      eapply H1 in B.
+      inv B.
+      * exfalso. exploit (step_internally_deterministic _ _ _ _ H12 H9 ); eauto. dcr; congruence.
+      * eexists; split. eauto. eapply f.
+        intros. Guarded.
+        eapply (produces_prefix_preserved (fun _ => True)); eauto.
+      * exfalso. eauto using activated_normal_star, star2.
+      * exfalso. exploit (step_internally_deterministic _ _ _ _ H8 H5 ); eauto. dcr; congruence.
+      *)
+      exfalso; clear_all; admit.
+    + intros. destruct evt.
+      assert (B:produces_prefix x (EEvtExtern call::nil)).
+      econstructor 2. eauto. eauto. econstructor 5.
+      assert (C:produces_prefix x2 (EEvtExtern call :: nil)). clear f; admit.
+      inv C.
+      * exfalso. eapply (no_activated_tau_step _ _ H12).
+      * eexists; split. eauto. eapply f.
+        intros. Guarded.
+        eapply (produces_prefix_preserved' (fun _ => True)); eauto.
+      * exfalso. eapply (activated_normal_star (star2_refl _ _) H7). eauto. eauto.
+      * exfalso. eapply (no_activated_tau_step _ _ H9).
+    + eauto.
+  - assert (diverges σ').
+    eapply (produces_diverges H1); eauto.
+    eapply bisim_complete_diverges; eauto.
+Qed.
+
+
+Inductive crashed : list extevent -> Prop :=
+| CrashCrash r
+  : r = None
+    -> crashed (EEvtTerminate r::nil)
+| CrashedStep e es
+  : crashed es
+    -> crashed (EEvt (EvtExtern e)::es).
+
+Lemma produces_not_crashed_crashdiverges S `{StateType S} S' `{StateType S'} (σ:S) (σ':S')
+: (forall L, not_crashed L -> produces_prefix σ' L -> produces_prefix σ L)
+  -> diverges σ -> crashdiverges σ'.
+Proof.
+  revert σ σ'.
+  cofix f; intros.
+  inv H2.
+  edestruct (@step_dec _ H0 σ').
+  inv H5; dcr.
+  destruct x.
+  - exfalso.
+    pose proof (diverges_produces_only_nil H2).
+    exploit H6. eapply H1. Focus 2.
+    econstructor 2. eexists; eauto. eauto. econstructor 4.
+    econstructor; econstructor.
+    congruence.
+  - econstructor. eapply H7.
+    eapply f; intros; try eapply H4.
+    + eapply produces_prefix_star2_silent'.
+      eapply (S_star2 EvtTau). eapply H3. econstructor.
+      eapply H1. eauto. econstructor; eauto.
+  - case_eq (result σ'); intros.
+    + exfalso.
+      exploit (diverges_produces_only_nil H2).
+      eapply H1. Focus 2.
+      econstructor 3; eauto. constructor.
+      eauto using not_crashed.
+      congruence.
+    + eapply crash_crashdiverges; eauto. econstructor.
+Qed.
+
+Lemma crashes_crashed S `{StateType S} S' `{StateType S'} (σ:S) (σ':S')
+:  (forall L : list extevent,
+      crashed L -> produces_prefix σ' L -> produces_prefix σ L)
+   -> crashes σ' -> crashes σ.
+Proof.
+  intros. destruct H2; dcr.
+  exploit producesPrefixTerm; eauto.
+  eapply H1 in X.
+  eapply produces_prefix_terminates in X. dcr.
+  eexists x0; intuition. eauto using crashed.
+Qed.
+
+(*
+Lemma produces_not_crashed_prefix_sim S `{StateType S} S' `{StateType S'} (σ:S) (σ':S')
+: (forall L, not_crashed L -> (produces_prefix σ L -> produces_prefix σ' L))
+  -> (forall L, crashed L -> (produces_prefix σ' L -> produces_prefix σ L))
+  -> sim σ σ'.
+Proof.
+  revert σ σ'.
+  cofix f; intros.
+  destruct (three_possibilities σ) as [A|[A|A]].
+  - dcr.
+    case_eq (result x); intros.
+    + assert (produces_prefix σ (EvtTerminate (result x)::nil)).
+      econstructor 3; eauto.
+      eapply H1 in H6; [|eauto using not_crashed].
+      eapply produces_prefix_terminates in H6. dcr.
+      econstructor 4; eauto.
+    + econstructor 3; eauto.
+  - dcr. inv H5; dcr.
+    assert (produces_prefix x1 nil) by econstructor 4.
+    exploit (produces_prefix_star_activated _ H4 H5 H6 H3).
+    eapply H1 in X;[| eauto using not_crashed].
+    eapply produces_prefix_extevent in X. dcr.
+    econstructor 2; eauto.
+    + intros.
+      assert (B:produces_prefix x (EEvt evt::nil)) by
+          (econstructor 2; eauto; econstructor 4).
+      eapply produces_not_crashed_silent_closed' in B; eauto.
+      inv B.
+      * exfalso. exploit (step_internally_deterministic _ _ _ _ H12 H10 ); eauto. dcr; congruence.
+      * eexists; split. eauto. eapply f.
+        eapply produces_prefix_preserved'; eauto.
+        intros; econstructor; eauto.
+        eapply produces_prefix_preserved'; eauto.
+        intros; econstructor; eauto.
+      * destruct evt; eauto using not_crashed.
+        exfalso. exploit (@step_internally_deterministic S _ ). eauto. eapply H6. dcr; congruence.
+    + intros.
+      assert (B:produces_prefix x2 (EEvt evt::nil)) by
+          (econstructor 2; eauto; econstructor 4).
+      pose proof (produces_not_crashed_silent_closed' H4 H8 H1); eauto.
+      inv B.
+      * exfalso. exploit (step_internally_deterministic _ _ _ _ H12 H10 ); eauto. dcr; congruence.
+      * eexists; split. eauto. eapply f.
+        eapply produces_prefix_preserved; eauto.
+        intros; econstructor; eauto.
+        eapply produces_prefix_preserved'; eauto.
+        intros; econstructor; eauto.
+      * destruct evt; eauto using not_crashed.
+        exfalso. eauto using no_activated_tau_step. Guarded.
+  - exploit (@produces_not_crashed_crashdiverges S _ S' _). eapply H1. eauto.
+    eapply crashdiverges_crashes_or_diverges in X. destruct X.
+    exfalso. eapply crashes_crashed in H3; eauto.
+    destruct H3; dcr.
+    eapply (diverges_never_terminates H6); eauto.
+    eapply sim_complete_diverges. eauto. eauto.
+Qed.
+
+Lemma sim_prefix {S} `{StateType S} {S'} `{StateType S'} (σ:S) (σ':S')
+: sim σ σ' -> forall L, produces_prefix σ' L -> produces_prefix σ L.
+Proof.
+  intros. general induction H2.
+  - eapply sim_sim' in H3.
+    eapply IHproduces_prefix; eauto.
+    eapply sim'_sim. eapply sim'_reduction_closed_2; eauto.
+    eapply (S_star2 _ _ H). eapply star2_refl.
+  - eapply sim_sim' in H4.
+    eapply sim'_activated_2 in H4; eauto.
+    dcr; intuition.
+    destruct evt.
+    + eapply produces_prefix_star2_silent; eauto.
+      edestruct H4; eauto. destruct H7.
+      econstructor 2. eauto. eapply H7.
+      eapply IHproduces_prefix; eauto.
+      eapply sim'_sim. eapply H9.
+    + exfalso; eapply (no_activated_tau_step _ H H1); eauto.
+    +
+  - case_eq (result σ'); intros.
+    eapply sim_sim' in H4. eapply sim'_terminate in H4; eauto.
+    destruct H4 as [? [? []]]. econstructor 3; [ | eauto | eauto]. congruence. congruence.
+  - econstructor 4.
+Qed.
+
+Lemma sim_traces S `{StateType S} S' `{StateType S'} (σ:S) (σ':S')
+: sim σ σ'
+  ->  (forall L, produces_prefix σ' L -> produces_prefix σ L).
+Proof.
+  intros.
+  general induction H2.
+  - eapply IHproduces_prefix.
+    eapply sim'_sim.
+    eapply sim'_reduction_closed. eapply sim_sim'. eapply H3. econstructor.
+    eapply (S_star2 EvtTau); eauto. constructor.
+  - destruct evt.
+    edestruct (@sim'_activated_2 S' _ σ S); eauto. eapply (sim_sim' H4).
+    intuition.
+    + inv H7. dcr. eapply produces_prefix_star_activated. eauto. eauto.
+*)
+Lemma three_possibilities' S `{StateType S} (σ:S)
+: { σ' | star2 step σ nil σ' /\ normal2 step σ' }
+  + { σ' | star2 step σ nil σ' /\ activated σ' }
+  + diverges σ.
+Proof.
+Admitted.
+
+Lemma activated_destr S `{StateType S} (σ:S)
+:  activated σ -> { ext : extern & { σ' | step σ (EvtExtern ext) σ' } }.
+Proof.
+  intros. admit.
+Qed.
+
+Lemma coproduces_trace S `{StateType S} (σ:S) : stream extevent.
+Proof.
+  revert σ. cofix f; intros σ.
+  destruct (three_possibilities' σ). destruct s.
+  - destruct s. eapply (sons (EvtTerminate (result x)) sil).
+  - destruct s. destruct a. eapply activated_destr in H1.
+    destruct H1. destruct s. refine (sons (EEvt (EvtExtern x0)) _).
+    eapply (f x1).
+  - eapply sil.
+Defined.
+
+Definition stream_match X (s:stream X) :=
+  match s with
+    | sil => sil
+    | sons A s => sons A s
+  end.
+
+Lemma stream_match_eq X (s:stream X)
+: s = stream_match s.
+Proof.
+  destruct s; reflexivity.
+Qed.
+
+Lemma coproduces_trace_sound S `{StateType S} (σ:S)
+: coproduces σ (coproduces_trace σ).
+Proof.
+  revert σ. cofix f; intros.
+  unfold coproduces_trace.
+  rewrite stream_match_eq; simpl.
+  case_eq (three_possibilities' σ); intros; simpl.
+  - destruct s. destruct s. econstructor; eauto.
+    + destruct s. destruct a.
+      destruct (activated_destr a). destruct s0.
+      econstructor. eauto. eauto. eauto. eapply f.
+  - econstructor 2. eauto.
+Qed.
+
+Lemma coproduces_total S `{StateType S} (σ:S)
+: exists L, coproduces σ L.
+Proof.
+  eexists. eapply coproduces_trace_sound.
+Qed.
+
+
+Inductive safe : stream extevent -> Prop :=
+| SafeTrm v
+  : safe (sons (EvtTerminate (Some v)) sil)
+| SafeDiv
+  : safe sil
+| SafeStep e es
+  : safe es
+    -> safe (sons e es).
+
+Lemma diverges_coproduces_only_sil S `{StateType S} S' `{StateType S'} (σ:S)
+: diverges σ -> (forall L, coproduces σ L -> L = sil).
+Proof.
+  intros. inv H2.
+  - exfalso. eapply (diverges_never_activated H4).
+    eapply diverges_reduction_closed; eauto.
+  - reflexivity.
+  - exfalso. eapply (diverges_never_terminates H5); eauto.
+Qed.
+
+CoInductive cocontinues X :
+
+Lemma coproduces_safe_bisim S `{StateType S} S' `{StateType S'} (σ:S) (σ':S')
+: (forall L, coproduces σ L -> coproduces σ' L)
+  -> sim σ σ'.
+Proof.
+  revert σ σ'.
+  cofix f; intros.
+  assert (exists L, safe L /\ coproduces σ L) by (exfalso; clear_all; admit).
+  dcr. inv H5.
+  - exploit H1. eauto. eauto.
+    inv X.
+    econstructor 2. eauto. eauto. eauto. eauto.
+    + intros.
+    +
+
+  - eapply H1 in H5. inv H5.
+    eapply sim_complete_diverges; eauto. eauto.
+  - case_eq (result σ'0); intros.
+    + exploit H1. eauto. eauto.
+      inv X.
+      econstructor 4. symmetry in H8. eapply H8.
+      eauto. eauto. eauto. eauto.
+    + econstructor 3; eauto.
+Qed.
+
+
+
+
+
+
+(*
+*** Local Variables: ***
+*** coq-load-path: (("../" "Lvc")) ***
+*** End: ***
+*)
