IL/Events.v
@@ -131,6 +131,27 @@ Proof.
       eapply IHstar2; eauto.
 Qed.
 
+Lemma star2_reach_normal2 X (R:X -> event -> X -> Prop) σ1 σ2a σ2b
+: star2 R σ1 nil σ2a
+  -> star2 R σ1 nil σ2b
+  -> internally_deterministic R
+  -> normal2 R σ2a
+  -> normal2 R σ2b
+  -> σ2a = σ2b.
+Proof.
+  intros.
+  general induction H0; eauto.
+  - general induction H.
+    + eauto.
+    + exfalso. eapply H3. firstorder.
+  - destruct y, yl; isabsurd; eauto. simpl in *.
+    inv H1.
+    + exfalso. eapply H3. do 2 eexists. eauto.
+    + destruct y, yl; isabsurd.
+      assert (x'0 = x'). eapply H2; eauto. subst.
+      eapply IHstar2; eauto.
+Qed.
+
 Lemma plus2_reach X (R:X -> event -> X -> Prop) σ1 σ2a σ2b
 : plus2 R σ1 nil σ2a
   -> plus2 R σ1 nil σ2b
